Reorganize and refactor things

extraction/examples/ErasureTests.v
@@ -25,18 +25,14 @@ Set Equations Transparent.
 
 Module flag_of_type_tests.
 Record type_flag_squashed := {
-  is_logical : bool;
-  is_sort : bool;
-  is_arity : bool }.
+                              is_logical : bool;
+                              is_sort : bool;
+                              is_arity : bool }.
 
 Program Definition flag_of_type_program (p : Ast.program)
   : result type_flag_squashed string :=
   let p := fix_program_universes p in
   let Σ := trans_global_decls p.1 in
-  G <- match check_wf_env_only_univs Σ with
-       | CorrectDecl a => ret a
-       | _ => Err "Could not check_wf_env_only_univs"
-       end;;
   f <- match flag_of_type (empty_ext Σ) _ [] (trans p.2) _ with
        | Checked a => ret a
        | TypeError te => Err "Could not get flag"
@@ -44,57 +40,68 @@ Program Definition flag_of_type_program (p : Ast.program)
   ret {| is_logical := Erasure.is_logical f;
          is_sort := if Erasure.is_sort f then true else false;
          is_arity := if Erasure.is_arity f then true else false |}.
-Next Obligation.
-  unfold trans_global.
-  simpl. unfold wf_ext, empty_ext. simpl.
-  unfold on_global_env_ext. destruct H0. constructor.
-  split; auto. simpl. todo "on_udecl on empty universe context".
-Qed.
-Next Obligation.
-  unfold trans_global.
-  simpl. unfold wf_ext, empty_ext. simpl.
-  unfold on_global_env_ext. destruct H0. todo "assuming well-typedness".
-Qed.
+Next Obligation. Admitted.
+Next Obligation. Admitted.
 
 MetaCoq Quote Recursively Definition ex1 := Type.
-Check eq_refl : ltac:(let x := eval vm_compute in (flag_of_type_program ex1) in exact x) =
-                Ok {| is_logical := false; is_sort := true; is_arity := true |}.
+Example ex1_test :
+  flag_of_type_program ex1 =
+  Ok {| is_logical := false; is_sort := true; is_arity := true |}.
+Proof. vm_compute. reflexivity. Qed.
 
 MetaCoq Quote Recursively Definition ex2 := nat.
-Check eq_refl : ltac:(let x := eval vm_compute in (flag_of_type_program ex2) in exact x) =
-                Ok {| is_logical := false; is_sort := false; is_arity := false |}.
+Example ex2_test :
+  flag_of_type_program ex2 =
+  Ok {| is_logical := false; is_sort := false; is_arity := false |}.
+Proof. vm_compute. reflexivity. Qed.
 
 MetaCoq Quote Recursively Definition ex3 := (nat -> nat).
-Check eq_refl : ltac:(let x := eval vm_compute in (flag_of_type_program ex3) in exact x) =
-                Ok {| is_logical := false; is_sort := false; is_arity := false |}.
+Example ex3_test :
+  flag_of_type_program ex3 =
+  Ok {| is_logical := false; is_sort := false; is_arity := false |}.
+Proof. vm_compute. reflexivity. Qed.
 
 MetaCoq Quote Recursively Definition ex4 := (forall A, A).
-Check eq_refl : ltac:(let x := eval vm_compute in (flag_of_type_program ex4) in exact x) =
-                Ok {| is_logical := false; is_sort := false; is_arity := false |}.
+Example ex4_test :
+  flag_of_type_program ex4 =
+  Ok {| is_logical := false; is_sort := false; is_arity := false |}.
+Proof. vm_compute. reflexivity. Qed.
 
 MetaCoq Quote Recursively Definition ex5 := (Prop).
-Check eq_refl : ltac:(let x := eval vm_compute in (flag_of_type_program ex5) in exact x) =
-                Ok {| is_logical := true; is_sort := true; is_arity := true |}.
+Example ex5_test :
+  flag_of_type_program ex5 =
+  Ok {| is_logical := true; is_sort := true; is_arity := true |}.
+Proof. vm_compute. reflexivity. Qed.
 
 MetaCoq Quote Recursively Definition ex5' := (forall n m: nat, Prop).
-Check eq_refl : ltac:(let x := eval vm_compute in (flag_of_type_program ex5') in exact x) =
-                Ok {| is_logical := true; is_sort := false; is_arity := true |}.
+Example ex5'_test :
+  flag_of_type_program ex5' =
+  Ok {| is_logical := true; is_sort := false; is_arity := true |}.
+Proof. vm_compute. reflexivity. Qed.
 
 MetaCoq Quote Recursively Definition ex6 := (Prop -> Type).
-Check eq_refl : ltac:(let x := eval vm_compute in (flag_of_type_program ex6) in exact x) =
-                Ok {| is_logical := false; is_sort := false; is_arity := true |}.
+Example ex6_test :
+  flag_of_type_program ex6 =
+  Ok {| is_logical := false; is_sort := false; is_arity := true |}.
+Proof. vm_compute. reflexivity. Qed.
 
 MetaCoq Quote Recursively Definition ex7 := (Type -> Prop).
-Check eq_refl : ltac:(let x := eval vm_compute in (flag_of_type_program ex7) in exact x) =
-                Ok {| is_logical := true; is_sort := false; is_arity := true |}.
+Example ex7_test :
+  flag_of_type_program ex7 =
+  Ok {| is_logical := true; is_sort := false; is_arity := true |}.
+Proof. vm_compute. reflexivity. Qed.
 
 MetaCoq Quote Recursively Definition ex8 := (False).
-Check eq_refl : ltac:(let x := eval vm_compute in (flag_of_type_program ex8) in exact x) =
-                Ok {| is_logical := true; is_sort := false; is_arity := false |}.
+Example ex8_test :
+  flag_of_type_program ex8 =
+  Ok {| is_logical := true; is_sort := false; is_arity := false |}.
+Proof. vm_compute. reflexivity. Qed.
 
 MetaCoq Quote Recursively Definition ex9 := (Fin.t 0 -> False).
-Check eq_refl : ltac:(let x := eval vm_compute in (flag_of_type_program ex9) in exact x) =
-                Ok {| is_logical := true; is_sort := false; is_arity := false |}.
+Example ex9_test :
+  flag_of_type_program ex9 =
+  Ok {| is_logical := true; is_sort := false; is_arity := false |}.
+Proof. vm_compute. reflexivity. Qed.
 End flag_of_type_tests.
 
 Module erase_type_tests.
@@ -109,25 +116,10 @@ Program Definition erase_type_program (p : Ast.program)
   : result (P.global_env * (list name * box_type)) erase_type_error :=
   let p := fix_program_universes p in
   let Σ := trans_global_decls p.1 in
-  G <- match check_wf_env_only_univs Σ with
-       | CorrectDecl a => ret a
-       | EnvError Σ err => Err (GeneralError
-                                  ("Could not check_wf_env_only_univs: "
-                                     ++ string_of_env_error Σ err))
-       end;;
-  t <- erase_type (empty_ext Σ) _ [] (Vector.nil _) (trans p.2) _ [];;
+  t <- erase_type SafeErasureFunction.erase (empty_ext Σ) _ [] (Vector.nil _) (trans p.2) _ [];;
   ret (Σ, t).
-Next Obligation.
-  unfold trans_global.
-  simpl. unfold wf_ext, empty_ext. simpl.
-  unfold on_global_env_ext. destruct H0. constructor.
-  split; auto. simpl. todo "on_udecl on empty universe context".
-Qed.
-Next Obligation.
-  unfold trans_global.
-  simpl. unfold wf_ext, empty_ext. simpl.
-  unfold on_global_env_ext. destruct H0. todo "assuming well-typedness".
-Qed.
+Next Obligation.  Admitted.
+Next Obligation.  Admitted.
 
 Definition is_arr (t : box_type) : bool :=
   match t with
@@ -153,24 +145,24 @@ Definition print_name (na : name) : string :=
 
 Definition print_box_type (Σ : P.global_env) (tvars : list name) :=
   fix f (bt : box_type) :=
-  match bt with
-  | TBox => "□"
-  | TAny => "𝕋"
-  | TArr dom codom => parens (negb (is_arr dom)) (f dom) ++ " → " ++ f codom
-  | TApp t1 t2 => f t1 ++ " " ++ parens (parenthesize_arg t2) (f t2)
-  | TVar i => match nth_error tvars i with
-              | Some na => print_name na
-              | None => "'a" ++ string_of_nat i
-              end
-  | TInd s =>
-    match @lookup_ind_decl (empty_ext Σ) s with
-    | Checked (decl; oib; _) => oib.(P.ind_name)
-    | TypeError te => "UndeclaredInductive("
-                        ++ string_of_kername s.(inductive_mind)
-                        ++ "," ++ string_of_nat s.(inductive_ind) ++ ")"
-    end
-  | TConst s => s.2
-  end.
+    match bt with
+    | TBox => "□"
+    | TAny => "𝕋"
+    | TArr dom codom => parens (negb (is_arr dom)) (f dom) ++ " → " ++ f codom
+    | TApp t1 t2 => f t1 ++ " " ++ parens (parenthesize_arg t2) (f t2)
+    | TVar i => match nth_error tvars i with
+                | Some na => print_name na
+                | None => "'a" ++ string_of_nat i
+                end
+    | TInd s =>
+      match @lookup_ind_decl (empty_ext Σ) s with
+      | Checked (decl; oib; _) => oib.(P.ind_name)
+      | TypeError te => "UndeclaredInductive("
+                          ++ string_of_kername s.(inductive_mind)
+                                                   ++ "," ++ string_of_nat s.(inductive_ind) ++ ")"
+      end
+    | TConst s => s.2
+    end.
 
 Definition print_type_vars (l : list name) :=
   String.concat " " (map print_name l).
@@ -184,135 +176,169 @@ Definition erase_and_print_type
   ret (print_type_vars tvars, print_box_type Σ tvars bt).
 
 MetaCoq Quote Recursively Definition ex1 := (forall (A B : Type) (a : A * B) (C : Type), A * B * C).
-Check eq_refl : ltac:(let x := eval vm_compute in (erase_and_print_type id ex1) in exact x) =
-                Ok ("A B C", "□ → □ → prod A B → □ → prod (prod A B) C").
+Example ex1_test :
+  erase_and_print_type id ex1 =
+  Ok ("A B C", "□ → □ → prod A B → □ → prod (prod A B) C").
+Proof. vm_compute. reflexivity. Qed.
 
 MetaCoq Quote Recursively Definition ex2 := (forall (A : Type) (P : A -> Prop), @sig A P).
-Check eq_refl : ltac:(let x := eval vm_compute in (erase_and_print_type id ex2) in exact x) =
-                Ok ("A", "□ → □ → sig A □").
+Example ex2_test :
+  erase_and_print_type id ex2 =
+  Ok ("A", "□ → □ → sig A □").
+Proof. vm_compute. reflexivity. Qed.
 
 MetaCoq Quote Recursively Definition ex3 := (forall (A : Type) (P : A -> Prop), { a : A | P a }).
-Check eq_refl : ltac:(let x := eval vm_compute in (erase_and_print_type id ex3) in exact x) =
-                Ok ("A", "□ → □ → sig A □").
+Example ex3_test :
+  erase_and_print_type id ex3 =
+  Ok ("A", "□ → □ → sig A □").
+Proof. vm_compute. reflexivity. Qed.
 
 MetaCoq Quote Recursively Definition ex4 := (forall (A B : Type) (f : A -> B) (n : nat),
-                                        Vector.t A n -> Vector.t B n).
-Check eq_refl : ltac:(let x := eval vm_compute in (erase_and_print_type id ex4) in exact x) =
-                Ok ("A B", "□ → □ → (A → B) → nat → t A 𝕋 → t B 𝕋").
+                                                Vector.t A n -> Vector.t B n).
+Example ex4_test :
+  erase_and_print_type id ex4 =
+  Ok ("A B", "□ → □ → (A → B) → nat → t A 𝕋 → t B 𝕋").
+Proof. vm_compute. reflexivity. Qed.
 
 MetaCoq Quote Recursively Definition ex5 :=
   (forall (A : Type),  list A -> list A -> 0 = 0 -> forall (B : Type), B -> A -> A).
-Check eq_refl : ltac:(let x := eval vm_compute in (erase_and_print_type id ex5) in exact x) =
-                Ok ("A B", "□ → list A → list A → □ → □ → B → A → A").
+Example ex5_test :
+  erase_and_print_type id ex5 =
+  Ok ("A B", "□ → list A → list A → □ → □ → B → A → A").
+Proof. vm_compute. reflexivity. Qed.
 
 (* Prenex form that we fail on *)
 MetaCoq Quote Recursively Definition ex6 :=
   (forall (A : Type), (forall A : Type, A -> A) -> A -> forall B : Type, B -> nat).
-Check eq_refl : ltac:(let x := eval vm_compute in (erase_and_print_type id ex6) in exact x) =
-                Err NotPrenex.
+Example ex6_test :
+  erase_and_print_type id ex6 =
+  Err NotPrenex.
+Proof. vm_compute. reflexivity. Qed.
 
 (** Erasing and deboxing *)
 MetaCoq Quote Recursively Definition ex7 :=
   (forall (A : Type), A -> forall (B : Type) (C : Type), B -> C).
-Check eq_refl : ltac:(let x := eval vm_compute in (erase_and_print_type id ex7) in exact x) =
-                Ok ("A B C", "□ → A → □ → □ → B → C").
+Example ex7_test :
+  erase_and_print_type id ex7 =
+  Ok ("A B C", "□ → A → □ → □ → B → C").
+Proof. vm_compute. reflexivity. Qed.
 
 (** Tesing mutual inductives *)
 Inductive tree (A : Set) : Set :=
   node : A -> forest A -> tree A
 with forest (A : Set) : Set :=
-    leaf : A -> forest A
-  | cons : tree A -> forest A -> forest A.
+  leaf : A -> forest A
+| cons : tree A -> forest A -> forest A.
 
 MetaCoq Quote Recursively Definition ex8 := (forall (A: Set), forest A -> tree A -> A).
-Check eq_refl : ltac:(let x := eval vm_compute in (erase_and_print_type id ex8) in exact x) =
-                Ok ("A", "□ → forest A → tree A → A").
+Example ex8_test :
+  erase_and_print_type id ex8 =
+  Ok ("A", "□ → forest A → tree A → A").
+Proof. vm_compute. reflexivity. Qed.
 
 (* We cannot currently handle the following even though we may want to be able to.
-   To handle this we would need to do deboxing simultaneously with erasure. *)
-MetaCoq Quote Recursively Definition ex9 := (forall (A : 0 = 0 -> Type) (B : Type), option (A eq_refl) -> B).
-Check eq_refl : ltac:(let x := eval vm_compute in (erase_and_print_type id ex9) in exact x) =
-                Err NotPrenex.
+ To handle this we would need to do deboxing simultaneously with erasure. *)
+MetaCoq Quote Recursively Definition ex9 :=
+  (forall (A : 0 = 0 -> Type) (B : Type), option (A eq_refl) -> B).
+Example ex9_test :
+  erase_and_print_type id ex9 =
+  Err NotPrenex.
+Proof. vm_compute. reflexivity. Qed.
 
 MetaCoq Quote Recursively Definition ex10 :=
   (forall (A : Type), (forall (B : Type), B -> B) -> A).
-Check eq_refl : ltac:(let x := eval vm_compute in (erase_and_print_type id ex10) in exact x) =
-                Err NotPrenex.
+Example ex10_test :
+  erase_and_print_type id ex10 =
+  Err NotPrenex.
+Proof. vm_compute. reflexivity. Qed.
 
 MetaCoq Quote Recursively Definition ex11 := (forall (A : Type), {n : nat | 0 < n} -> A).
-Check eq_refl : ltac:(let x := eval vm_compute in (erase_and_print_type id ex11) in exact x) =
-                Ok ("A", "□ → sig nat □ → A").
+Example ex11_test :
+  erase_and_print_type id ex11 =
+  Ok ("A", "□ → sig nat □ → A").
+Proof. vm_compute. reflexivity. Qed.
 
 MetaCoq Quote Recursively Definition ex12 := (forall (A : Type) (P : A -> Prop), unit).
-Check eq_refl : ltac:(let x := eval vm_compute in (erase_and_print_type id ex12) in exact x) =
-                Ok ("A", "□ → □ → unit").
+Example ex12_test :
+  erase_and_print_type id ex12 =
+  Ok ("A", "□ → □ → unit").
+Proof. vm_compute. reflexivity. Qed.
 
 MetaCoq Quote Recursively Definition ex13 := (let p := (nat, unit) in fst p × snd p).
-Check eq_refl : ltac:(let x := eval vm_compute in (erase_and_print_type id ex13) in exact x) =
-                Ok ("", "prod (fst □ □ 𝕋) (snd □ □ 𝕋)").
+Example ex13_test :
+  erase_and_print_type id ex13 =
+  Ok ("", "prod (fst □ □ 𝕋) (snd □ □ 𝕋)").
+Proof. vm_compute. reflexivity. Qed.
 
 MetaCoq Quote Recursively Definition ex14 := (let t := nat in t).
-Check eq_refl : ltac:(let x := eval vm_compute in (erase_and_print_type id ex14) in exact x) =
-                Ok ("", "nat").
+Example ex14_test :
+  erase_and_print_type id ex14 =
+  Ok ("", "nat").
+Proof. vm_compute. reflexivity. Qed.
 
 MetaCoq Quote Recursively Definition ex15 := ((fix f n := match n with
-                                                  | 0 => nat
-                                                  | S n => nat -> f n
-                                                  end) 5).
-Check eq_refl : ltac:(let x := eval vm_compute in (erase_and_print_type id ex15) in exact x) =
-                Ok ("", "nat → nat → nat → nat → nat → nat").
+                                                          | 0 => nat
+                                                          | S n => nat -> f n
+                                                          end) 5).
+Example ex15_test :
+  erase_and_print_type id ex15 =
+  Ok ("", "nat → nat → nat → nat → nat → nat").
+Proof. vm_compute. reflexivity. Qed.
 
 MetaCoq Quote Recursively Definition ex16 := (Type -> Type).
-Check eq_refl : ltac:(let x := eval vm_compute in (erase_and_print_type id ex16) in exact x) =
-                Ok ("_", "□ → □").
+Example ex16_test :
+  erase_and_print_type id ex16 =
+  Ok ("_", "□ → □").
+Proof. vm_compute. reflexivity. Qed.
 
 MetaCoq Quote Recursively Definition ex17 := (Type -> Prop).
-Check eq_refl : ltac:(let x := eval vm_compute in (erase_and_print_type id ex17) in exact x) =
-                Ok ("", "□").
+Example ex17_test :
+  erase_and_print_type id ex17 =
+  Ok ("", "□").
+Proof. vm_compute. reflexivity. Qed.
 
 MetaCoq Quote Recursively Definition ex18 := (False).
-Check eq_refl : ltac:(let x := eval vm_compute in (erase_and_print_type id ex18) in exact x) =
-                Ok ("", "□").
+Example ex18_test :
+  erase_and_print_type id ex18 =
+  Ok ("", "□").
+Proof. vm_compute. reflexivity. Qed.
 
 MetaCoq Quote Recursively Definition ex19 := (Fin.t 0 -> False).
-Check eq_refl : ltac:(let x := eval vm_compute in (erase_and_print_type id ex19) in exact x) =
-                Ok ("", "□").
-
+Example ex19_test :
+  erase_and_print_type id ex19 =
+  Ok ("", "□").
+Proof. vm_compute. reflexivity. Qed.
 End erase_type_tests.
 
 Module erase_ind_arity_tests.
 Program Definition erase_arity_program (p : Ast.program)
-  : result (list oib_type_var) string :=
+: result (list oib_type_var) string :=
   let p := fix_program_universes p in
   let Σ := trans_global_decls p.1 in
-  G <- match check_wf_env_only_univs Σ with
-       | CorrectDecl a => ret a
-       | _ => Err "Could not check_wf_env_only_univs"
-       end;;
-  wrap_typing_result (erase_ind_arity (empty_ext Σ) _ [] (trans p.2) _)
+  wrap_typing_result (erase_ind_arity SafeErasureFunction.erase (empty_ext Σ) _ [] (trans p.2) _)
                      (string_of_type_error (empty_ext Σ)).
-Next Obligation.
-  Admitted.
-Next Obligation.
-  Admitted.
+Next Obligation. Admitted.
+Next Obligation. Admitted.
 
 MetaCoq Quote Recursively Definition ex1 := (forall (A : Type), A -> A -> Prop).
-Check eq_refl : ltac:(let x := eval vm_compute in (erase_arity_program ex1) in exact x) =
-                Ok
-                  [{| tvar_name := nNamed "A";
-                      tvar_is_logical := false;
-                      tvar_is_arity := true;
-                      tvar_is_sort := true |};
-                  {|
-                    tvar_name := nAnon;
-                    tvar_is_logical := false;
-                    tvar_is_arity := false;
-                    tvar_is_sort := false |};
-                  {|
-                    tvar_name := nAnon;
-                    tvar_is_logical := false;
-                    tvar_is_arity := false;
-                    tvar_is_sort := false |}].
+Example ex1_test :
+  erase_arity_program ex1 =
+  Ok
+    [{| tvar_name := nNamed "A";
+        tvar_is_logical := false;
+        tvar_is_arity := true;
+        tvar_is_sort := true |};
+    {|
+      tvar_name := nAnon;
+      tvar_is_logical := false;
+      tvar_is_arity := false;
+      tvar_is_sort := false |};
+    {|
+      tvar_name := nAnon;
+      tvar_is_logical := false;
+      tvar_is_arity := false;
+      tvar_is_sort := false |}].
+Proof. vm_compute. reflexivity. Qed.
 End erase_ind_arity_tests.
 
 Module erase_ind_tests.
@@ -330,8 +356,8 @@ Definition parenthesize_ctor_type (bt : box_type) : bool :=
   end.
 
 Definition print_one_inductive_body
-         (Σ : global_env)
-         (oib : ExAst.one_inductive_body) : string :=
+           (Σ : global_env)
+           (oib : ExAst.one_inductive_body) : string :=
   let print_ctor_type bt :=
       " " ++ parens
           (negb (parenthesize_ctor_type bt))
@@ -352,7 +378,7 @@ Definition print_inductive (Σ : global_env) (mib : ExAst.mutual_inductive_body)
 Axiom assume_wellformed : forall {X}, X.
 Axiom cannot_happen : forall {X}, X.
 Definition erase_and_print_ind_prog (p : Ast.program)
-           : result string erase_ind_error :=
+  : result string erase_ind_error :=
   let p := fix_program_universes p in
   let Σ := trans_global_decls p.1 in
   match trans p.2 with
@@ -360,6 +386,7 @@ Definition erase_and_print_ind_prog (p : Ast.program)
     match List.find (fun '(kn, _) => eq_kername kn (inductive_mind ind)) Σ with
     | Some (kn, P.InductiveDecl mib) =>
       inder <- erase_ind
+                 SafeErasureFunction.erase
                  (Σ, ind_universes mib) assume_wellformed
                  (inductive_mind ind) mib assume_wellformed;;
       ret (print_inductive Σ inder)
@@ -369,93 +396,113 @@ Definition erase_and_print_ind_prog (p : Ast.program)
   end.
 
 MetaCoq Quote Recursively Definition ex1 := nat.
-Check eq_refl : ltac:(let x := eval vm_compute in (erase_and_print_ind_prog ex1) in exact x) =
-                Ok ("data nat" ++ nl ++
-                    "| O" ++ nl ++
-                    "| S nat").
+Example ex1_test :
+  erase_and_print_ind_prog ex1 = Ok <$
+"data nat";
+"| O";
+"| S nat" $>.
+Proof. vm_compute. reflexivity. Qed.
 
 MetaCoq Quote Recursively Definition ex2 := sig.
-Check eq_refl : ltac:(let x := eval vm_compute in (erase_and_print_ind_prog ex2) in exact x) =
-                Ok ("data sig A P" ++ nl ++
-                    "| exist □ □ A □").
+Example ex2_test :
+  erase_and_print_ind_prog ex2 = Ok <$
+"data sig A P";
+"| exist □ □ A □" $>.
+Proof. vm_compute. reflexivity. Qed.
 
 MetaCoq Quote Recursively Definition ex3 := list.
-Check eq_refl : ltac:(let x := eval vm_compute in (erase_and_print_ind_prog ex3) in exact x) =
-                Ok ("data list A" ++ nl ++
-                    "| nil □" ++ nl ++
-                    "| cons □ A (list A)").
+Example ex3_test :
+  erase_and_print_ind_prog ex3 = Ok <$
+"data list A";
+"| nil □";
+"| cons □ A (list A)" $>.
+Proof. vm_compute. reflexivity. Qed.
 
 MetaCoq Quote Recursively Definition ex4 := option.
-Check eq_refl : ltac:(let x := eval vm_compute in (erase_and_print_ind_prog ex4) in exact x) =
-                Ok ("data option A" ++ nl ++
-                    "| Some □ A" ++ nl ++
-                    "| None □").
+Example ex4_test :
+  erase_and_print_ind_prog ex4 = Ok <$
+"data option A";
+"| Some □ A";
+"| None □" $>.
+Proof. vm_compute. reflexivity. Qed.
 
 MetaCoq Quote Recursively Definition ex5 := Vector.t.
-Check eq_refl : ltac:(let x := eval vm_compute in (erase_and_print_ind_prog ex5) in exact x) =
-                Ok ("data t A _" ++ nl ++
-                    "| nil □" ++ nl ++
-                    "| cons □ A nat (t A 𝕋)").
+Example ex5_test :
+  erase_and_print_ind_prog ex5 = Ok <$
+"data t A _";
+"| nil □";
+"| cons □ A nat (t A 𝕋)" $>.
+Proof. vm_compute. reflexivity. Qed.
 
 Inductive tree (A : Set) : Set :=
   node : A -> forest A -> tree A
 with forest (A : Set) : Set :=
-    leaf : A -> forest A
-  | cons : tree A -> forest A -> forest A.
+  leaf : A -> forest A
+| cons : tree A -> forest A -> forest A.
 MetaCoq Quote Recursively Definition ex6 := tree.
-Check eq_refl : ltac:(let x := eval vm_compute in (erase_and_print_ind_prog ex6) in exact x) =
-                Ok ("data tree A" ++ nl ++
-                    "| node □ A (forest A)" ++ nl ++
-                    "data forest A" ++ nl ++
-                    "| leaf □ A" ++ nl ++
-                    "| cons □ (tree A) (forest A)").
+Example ex6_test :
+  erase_and_print_ind_prog ex6 = Ok <$
+"data tree A";
+"| node □ A (forest A)";
+"data forest A";
+"| leaf □ A";
+"| cons □ (tree A) (forest A)" $>.
+Proof. vm_compute. reflexivity. Qed.
 
 Inductive Env :=
-     | EnvCtr : MEnv -> MTEnv -> Env
+| EnvCtr : MEnv -> MTEnv -> Env
 with MEnv :=
-     | MEnvCtr : False -> list Mod -> MEnv
+| MEnvCtr : False -> list Mod -> MEnv
 with MTEnv :=
-     | MTEnvCtr : list MTy -> MTEnv
+| MTEnvCtr : list MTy -> MTEnv
 with Mod :=
-     | NonParamMod : Env -> Mod
-     | Ftor : Env -> MTy -> Mod
+| NonParamMod : Env -> Mod
+| Ftor : Env -> MTy -> Mod
 with MTy :=
-     | MSigma : Mod -> MTy.
+| MSigma : Mod -> MTy.
 MetaCoq Quote Recursively Definition ex7 := Env.
-Check eq_refl : ltac:(let x := eval vm_compute in (erase_and_print_ind_prog ex7) in exact x) =
-                Ok ("data Env" ++ nl ++
-                    "| EnvCtr MEnv MTEnv" ++ nl ++
-                    "data MEnv" ++ nl ++
-                    "| MEnvCtr □ (list Mod)" ++ nl ++
-                    "data MTEnv" ++ nl ++
-                    "| MTEnvCtr (list MTy)" ++ nl ++
-                    "data Mod" ++ nl ++
-                    "| NonParamMod Env" ++ nl ++
-                    "| Ftor Env MTy" ++ nl ++
-                    "data MTy" ++ nl ++
-                    "| MSigma Mod").
+Example ex7_test :
+  erase_and_print_ind_prog ex7 = Ok <$
+"data Env";
+"| EnvCtr MEnv MTEnv";
+"data MEnv";
+"| MEnvCtr □ (list Mod)";
+"data MTEnv";
+"| MTEnvCtr (list MTy)";
+"data Mod" ++ nl ++
+"| NonParamMod Env";
+"| Ftor Env MTy";
+"data MTy";
+"| MSigma Mod" $>.
+Proof. vm_compute. reflexivity. Qed.
 
 Inductive Weird (A : Type) : Type :=
 | Nil
 | Cons (a : A) (w : Weird (A * A)).
 
 MetaCoq Quote Recursively Definition ex8 := Weird.
-Check eq_refl : ltac:(let x := eval vm_compute in (erase_and_print_ind_prog ex8) in exact x) =
-                Ok ("data Weird A" ++ nl ++
-                    "| Nil □" ++ nl ++
-                    "| Cons □ A (Weird (prod A A))").
+Example ex8_test :
+  erase_and_print_ind_prog ex8 = Ok <$
+"data Weird A";
+"| Nil □";
+"| Cons □ A (Weird (prod A A))" $>.
+Proof. vm_compute. reflexivity. Qed.
 
 Inductive IndexedList : Type -> Type :=
 | inil : forall T, IndexedList T
 | icons : forall T, T -> IndexedList T -> IndexedList T.
 
 MetaCoq Quote Recursively Definition ex9 := IndexedList.
-Check eq_refl : ltac:(let x := eval vm_compute in (erase_and_print_ind_prog ex9) in exact x) =
-                Err (EraseIndBodyError "IndexedList" (CtorUnmappedTypeVariables "inil")).
+Example ex9_test :
+  erase_and_print_ind_prog ex9 =
+  Err (EraseIndBodyError "IndexedList" (CtorUnmappedTypeVariables "inil")).
+Proof. vm_compute. reflexivity. Qed.
 
 MetaCoq Quote Recursively Definition ex10 := Monad.
-Check eq_refl : ltac:(let x := eval vm_compute in (erase_and_print_ind_prog ex10) in exact x) =
-                Err (EraseIndBodyError "Monad" (EraseCtorError "Build_Monad" NotPrenex)).
+Example ex10_test :
+  erase_and_print_ind_prog ex10 =
+  Err (EraseIndBodyError "Monad" (EraseCtorError "Build_Monad" NotPrenex)).
+Proof. vm_compute. reflexivity. Qed.
 
 Inductive ManyParamsInd (A : Type) (P : Prop) (Q : Prop) (B : Type) :=
   MPIConstr : P -> A -> B -> ManyParamsInd A P Q B.
@@ -463,10 +510,10 @@ Inductive ManyParamsInd (A : Type) (P : Prop) (Q : Prop) (B : Type) :=
 MetaCoq Quote Recursively Definition ex11 := ManyParamsInd.
 
 Example ManyParamsInd_test :
-  erase_and_print_ind_prog ex11 =
-  Ok <$ "data ManyParamsInd A P Q B";
-        "| MPIConstr □ □ □ □ □ A B" $>.
-Proof. reflexivity. Qed.
+  erase_and_print_ind_prog ex11 = Ok <$
+"data ManyParamsInd A P Q B";
+"| MPIConstr □ □ □ □ □ A B" $>.
+Proof. vm_compute. reflexivity. Qed.
 
 (* [Q] is non-arity parameter *)
 Inductive ManyParamsIndNonArity (A : Type) (P : Prop) (Q : True) (B : Type) :=
@@ -476,10 +523,10 @@ Inductive ManyParamsIndNonArity (A : Type) (P : Prop) (Q : True) (B : Type) :=
 MetaCoq Quote Recursively Definition ex12 := ManyParamsIndNonArity.
 
 Example ManyParamsIndNonArity_test:
-  erase_and_print_ind_prog ex12 =
-  Ok <$ "data ManyParamsIndNonArity A P Q B";
-        "| MPINAConstr1 □ □ □ □ □ A B";
-        "| MPINAConstr2 □ □ □ □ □ (list □) (prod A B)" $>.
+  erase_and_print_ind_prog ex12 = Ok <$
+"data ManyParamsIndNonArity A P Q B";
+"| MPINAConstr1 □ □ □ □ □ A B";
+"| MPINAConstr2 □ □ □ □ □ (list □) (prod A B)" $>.
 Proof. vm_compute. reflexivity. Qed.
 
 Inductive PropTypeVarInCtor :=
@@ -487,9 +534,9 @@ Inductive PropTypeVarInCtor :=
 MetaCoq Quote Recursively Definition ex13 := PropTypeVarInCtor.
 
 Example PropTypeVarInCtor_test :
-  erase_and_print_ind_prog ex13 =
-  Ok <$ "data PropTypeVarInCtor";
-        "| ex13_ctor □" $>.
+  erase_and_print_ind_prog ex13 = Ok <$
+"data PropTypeVarInCtor";
+"| ex13_ctor □" $>.
 Proof. vm_compute. reflexivity. Qed.
 
 Inductive IndWithIndex : nat -> Type :=
@@ -500,5 +547,4 @@ Example IndWithIndex_test :
   erase_and_print_ind_prog ex14 =
   Err (EraseIndBodyError "IndWithIndex" (CtorUnmappedTypeVariables "ex14_ctor")).
 Proof. vm_compute. reflexivity. Qed.
-
 End erase_ind_tests.
