extraction/examples/CounterCertifiedExtraction.v
@@ -167,7 +167,7 @@ Definition TT_rename :=
     that removes application of boxes to constants and constructors. *)
 
 Time MetaCoq Run
-     (t <- liquitidy_extraction PREFIX TT_remap TT_rename COUNTER_MODULE ;;
+     (t <- liquidity_extraction PREFIX TT_remap TT_rename COUNTER_MODULE ;;
       tmDefinition COUNTER_MODULE.(lmd_module_name) t).
 
 Print liquidity_counter.
