extraction/theories/ExtractionCorrectness.v
@@ -1,0 +1,1 @@
+From ConCert.Extraction Require Import Extraction.
