extraction/theories/SpecializeChainBase.v
@@ -1,0 +1,301 @@
+(* These next functions deal with specializing globals that might
+   refer to a ChainBase variable in the context. They work by
+   replacing uses of it with the specified term, and by removing it
+   from applications. For example:
+   Inductive Foo (cb : ChainBase) := ctor (addr : Address cb).
+   Definition a (cb : ChainBase) (n : nat) := n.
+   Definition b (cb : ChainBase) (addr : Foo cb) (n : N) :=
+     a cb (N.to_nat n).
+
+   becomes
+   Inductive Foo := ctor (addr : Address replacement_term).
+   Definition a (n : nat) := n.
+   Definition b (addr : Foo) (n : N) :=
+     a (N.to_nat n).
+
+   Note: Only specializes ChainBase when it is the very first abstraction.  *)
+
+From ConCert.Execution Require Import Blockchain.
+From ConCert.Execution Require Import Serializable.
+From ConCert.Extraction Require Import Common.
+From ConCert.Extraction Require Import ResultMonad.
+From Coq Require Import List.
+From Coq Require Import String.
+From MetaCoq.Template Require Import BasicAst.
+From MetaCoq.Template Require Import Loader.
+From MetaCoq.Template Require Import monad_utils.
+From MetaCoq.Template Require Import utils.
+From MetaCoq.PCUIC Require Import PCUICAst.
+
+Import MonadNotation.
+Local Open Scope string.
+
+Definition ChainBase_kername : kername :=
+  <%% ChainBase %%>.
+
+Section ChainBaseSpecialization.
+  Context (replacement_term : term).
+
+  Definition contains (n : kername) : list kername -> bool :=
+    existsb (eq_kername n).
+
+  Inductive VarInfo :=
+  (* this var is a ChainBase that should be replaced by the replacement term *)
+  | replace
+  (* this var has type ChainBase -> ... and its first argument should be removed *)
+  | specialize
+  | none.
+
+  Fixpoint specialize_term
+            (specialized : list kername) : list VarInfo -> term -> result term string :=
+    fix f Γ t :=
+      match t with
+      | tRel n =>
+        vi <- result_of_option (nth_error Γ n) "Unbound tRel";;
+        match vi with
+        | replace => ret replacement_term
+        | specialize => Err "Unapplied tRel that should be specialized appears in term"
+        | none => ret t
+        end
+      | tVar _ => ret t
+      | tEvar n ts =>
+        ts <- monad_map (f Γ) ts;;
+        ret (tEvar n ts)
+      | tSort univ =>
+        ret t
+      | tProd name ty body =>
+        ty <- f Γ ty;;
+        body <- f (none :: Γ) body;;
+        ret (tProd name ty body)
+      | tLambda name ty body =>
+        ty <- f Γ ty;;
+        body <- f (none :: Γ) body;;
+        ret (tLambda name ty body)
+      | tLetIn name val val_ty body =>
+        val <- f Γ val;;
+        val_ty <- f (none :: Γ) val_ty;;
+        body <- f (none :: Γ) body;;
+        ret (tLetIn name val val_ty body)
+      | tApp (tConst name _ as head) arg
+      | tApp (tInd {| inductive_mind := name |} _ as head) arg
+      | tApp (tConstruct {| inductive_mind := name |} _ _ as head) arg =>
+        if contains name specialized then
+          ret head
+        else
+          arg <- f Γ arg;;
+          ret (tApp head arg)
+      | tApp (tRel i as head) arg =>
+        vi <- result_of_option (nth_error Γ i) "Unbound tRel";;
+        match vi with
+        | replace => Err "Unexpected application"
+        | specialize => ret (tRel (i - 1)) (* removed chain base inbetween, hacky *)
+        | none => arg <- f Γ arg;;
+                  ret (tApp head arg)
+        end
+      | tApp head arg =>
+        head <- f Γ head;;
+        arg <- f Γ arg;;
+        ret (tApp head arg)
+      | tConst name _
+      | tInd {| inductive_mind := name |} _
+      | tConstruct {| inductive_mind := name |} _ _ =>
+        if contains name specialized then
+          Err ("Unapplied '"
+                  ++ string_of_kername name
+                  ++ "' (or constructor) appears in term; this needs to be specialized")
+        else
+          ret t
+      | tCase ind ret_ty disc brs =>
+        ret_ty <- f Γ ret_ty;;
+        disc <- f Γ disc;;
+        brs <- monad_map (fun '(ar, t) => t <- f Γ t;; ret (ar, t)) brs;;
+        ret (tCase ind ret_ty disc brs)
+      | tProj proj body =>
+        body <- f Γ body;;
+        ret (tProj proj body)
+      | tFix defs i =>
+        let Γ := (repeat none (List.length defs) ++ Γ)%list in
+        defs <- monad_map (fun (d : def term) =>
+                              dtype <- f Γ (dtype d);;
+                              dbody <- f Γ (dbody d);;
+                              ret {| dname := dname d;
+                                    dtype := dtype;
+                                    dbody := dbody;
+                                    rarg := rarg d |}) defs;;
+        ret (tFix defs i)
+      | tCoFix defs i =>
+        let Γ := (repeat none (List.length defs) ++ Γ)%list in
+        defs <- monad_map (fun (d : def term) =>
+                              dtype <- f Γ (dtype d);;
+                              dbody <- f Γ (dbody d);;
+                              ret {| dname := dname d;
+                                    dtype := dtype;
+                                    dbody := dbody;
+                                    rarg := rarg d |}) defs;;
+        ret (tCoFix defs i)
+      end.
+
+  Definition specialize_body
+              (specialized : list kername)
+              (name : kername)
+              (Γ : list VarInfo)
+              (remove : bool)
+              (t : term) : result term string :=
+    match remove, t with
+    | true, tLambda _ _ body =>
+      map_error (fun s => "While specializing body in " ++ string_of_kername name ++ ": " ++ s)
+                (specialize_term specialized (replace :: Γ) body)
+
+    | true, _ => Err ("Expected lambda in " ++ string_of_kername name ++ ", got" ++ nl ++ PUtil.string_of_term t)
+    | false, _ => specialize_term specialized Γ t
+    end.
+
+  Definition specialize_type
+              (specialized : list kername)
+              (name : kername)
+              (Γ : list VarInfo)
+              (remove : bool)
+              (t : term) : result term string :=
+    match remove, t with
+    | true, tProd _ _ body =>
+      map_error (fun s => "While specializing type in " ++ string_of_kername name ++ ": " ++ s)
+                (specialize_term specialized (replace :: Γ) body)
+
+    | true, _ => Err ("Expected product in " ++ string_of_kername name ++ ", got" ++ nl ++ PUtil.string_of_term t)
+    | false, _ => specialize_term specialized Γ t
+    end.
+
+  Definition specialize_decl
+              (specialized : list kername)
+              (kn : kername)
+              (decl : global_decl) : result (list kername * global_decl) string :=
+    match decl with
+    | ConstantDecl cst =>
+      let remove := match cst_type cst with
+                    | tProd _ (tInd ind _) _ =>
+                      eq_kername (inductive_mind ind) (ChainBase_kername)
+                    | _ => false
+                    end in
+
+      type <- specialize_type specialized kn [] remove (cst_type cst);;
+      body <- match cst_body cst with
+              | Some body => body <- specialize_body specialized kn [] remove body;;
+                              ret (Some body)
+              | None => ret None
+              end;;
+
+      ret (if remove then kn :: specialized else specialized,
+            ConstantDecl
+              {| cst_type := type;
+                cst_body := body;
+                cst_universes := cst_universes cst |})
+
+    | InductiveDecl mib =>
+      let params := rev (ind_params mib) in
+      let remove := match params with
+                    | {| decl_type := tInd ind _ |} :: _ =>
+                      eq_kername (inductive_mind ind) ChainBase_kername
+                    | _ => false
+                    end in
+      let go '(params, Γ) cdecl :=
+          body <- match decl_body cdecl with
+                  | Some body =>
+                    body <- map_error (fun s => "While specializing param body of "
+                                                  ++ string_of_kername kn ++ ": " ++ s)
+                                      (specialize_term specialized Γ body);;
+                    ret (Some body)
+                  | None => ret None
+                  end;;
+          type <- map_error (fun s => "While specializing param type of "
+                                        ++ string_of_kername kn ++ ": " ++ s)
+                            (specialize_term specialized Γ (decl_type cdecl));;
+          let cdecl :=
+              {| decl_name := decl_name cdecl;
+                  decl_body := body;
+                  decl_type := type |} in
+          ret (params ++ [cdecl], none :: Γ)%list in
+      '(params, _) <- monad_fold_left
+                        go
+                        (if remove then tl params else params)
+                        ([], if remove then [replace] else []);;
+      let params := rev params in
+      let go oib :=
+          type <- specialize_type specialized (kn.1, ind_name oib) [] remove (ind_type oib);;
+          (* Context with all mutually inductive types added,
+            specializing them if we removed an abstraction.
+            Ctors themselves will be abstracted over parameters. *)
+          let ctorΓ := repeat (if remove then specialize else none)
+                              (List.length (ind_bodies mib)) in
+          ctors <- monad_map
+                      (fun '(name, t, n) =>
+                        t <- specialize_type specialized (kn.1, name) ctorΓ remove t;;
+                        ret (name, t, n))
+                      (ind_ctors oib);;
+          (* Projections are just the type of the data value and
+            checked in a context with parameters and the record value
+            itself *)
+          let projΓ := none :: repeat none (List.length params) in
+          projs <- monad_map
+                      (fun '(name, t) =>
+                        t <- map_error (fun s => "While specializing projection "
+                                                    ++ name ++ ": " ++ s)
+                                        (specialize_term specialized projΓ t);;
+                        ret (name, t))
+                      (ind_projs oib);;
+          ret
+            {| ind_name := ind_name oib;
+                ind_type := type;
+                ind_kelim := ind_kelim oib;
+                ind_ctors := ctors;
+                ind_projs := projs; |} in
+      bodies <- monad_map go (ind_bodies mib);;
+      ret (if remove then kn :: specialized else specialized,
+            InductiveDecl
+              {| ind_finite := ind_finite mib;
+                ind_npars := List.length params;
+                ind_params := params;
+                ind_bodies := bodies;
+                ind_universes := ind_universes mib;
+                ind_variance := ind_variance mib; |})
+    end.
+End ChainBaseSpecialization.
+
+Definition axiomatized_ChainBase := 0.
+
+Definition axiomatized_ChainBase_kername : kername :=
+  <%% axiomatized_ChainBase %%>.
+
+Definition axiomatized_ChainBase_decl : global_decl :=
+  ConstantDecl
+    {| cst_type :=
+          tInd
+            {| inductive_mind := ChainBase_kername;
+              inductive_ind := 0; |}
+            [];
+        cst_body := None;
+        cst_universes := Monomorphic_ctx ContextSet.empty |}.
+
+(* Specialize ChainBase away in all definitions in an environment.
+    Note: this will also add an axiomatized chain base to the environment. *)
+Fixpoint specialize_env_rev (Σ : global_env) : result global_env string :=
+  match Σ with
+  | [] => ret []
+  | (name, decl) :: Σ =>
+    if eq_kername name ChainBase_kername then
+      let rep_term := tConst axiomatized_ChainBase_kername [] in
+      let go '(specialized, newΣ) '(name, decl) :=
+          '(specialized, decl) <- specialize_decl rep_term specialized name decl;;
+          ret (specialized, (name, decl) :: newΣ) in
+      '(_, newΣ_rev) <- monad_fold_left go Σ ([], []);;
+      ret ((name, decl)
+              :: (axiomatized_ChainBase_kername, axiomatized_ChainBase_decl)
+              :: rev newΣ_rev)
+    else
+      Σ <- specialize_env_rev Σ;;
+      ret ((name, decl) :: Σ)
+  end.
+
+(* TODO: There are many reverses here, we should improve this. *)
+Definition specialize_ChainBase_env (Σ : global_env) : result global_env string :=
+  Σrev <- specialize_env_rev (List.rev Σ);;
+  ret (List.rev Σrev).
